\question 

\begin{parts}

\part Show that the composition of homotopy equivalences $X \rightarrow Y$ and
$Y \rightarrow Z$ is a homotopy equivalence $X \rightarrow Z$. Deduce that
homotopy equivalence is an equivalence relation.

\begin{solution}
%
Suppose that $f_1:X \rightarrow Y$ and $f_2:Y \rightarrow Z$ are homotopy
equivalences with homotopy inverses $g_1, g_2$, respectively. We want to show
that $f_2f_1: X \rightarrow Z$ is a homotopy equivalence. Note that $g_1g_2:Z
\rightarrow X$ for which

\[(f_2f_1) \circ (g_1g_2) = f_2 \circ (f_1g_1) \circ g_2 \simeq f_2 \circ
\mathbb{1}_Y \circ g_2 = f_2g_2 \simeq \mathbb{1}_Z, \] and
\[
(g_1g_2) \circ (f_2f_1) = g_1 \circ (g_2f_2) \circ f_1 \simeq g_1 \circ 
\mathbb{1}_Z \circ f_1 = g_1f_1 \simeq \mathbb{1}_X.
\]

\end{solution}

\part Show that the relation of homotopy among maps $X \rightarrow Y$ is an 
equivalence relation.

\begin{solution}

This relation is \textit{reflexive} because $f:X \rightarrow Y$ is homotopic to
itself by the identity homotopy: $F(x,t) = x$.

The relation is \textit{symmetric} because if $f,g:X \rightarrow Y$ are
homotopic and $f \simeq g$ by a homotopy $\varphi_t$, then $g \simeq f$ by the
inverse homotopy $\varphi_t^{-1}$, defined by $\varphi_t^{-1}(x) =
\varphi_{(1-t)}(x)$.

Finally, the relation is \textit{transitive}. To show this, suppose that $F:X
\times I \rightarrow Y$ is a homotopy connecting $f$ to $g$ and that $G: X
\times I \rightarrow Y$ is a homotopy connecting $g$ to $h$, where $f$, $g$, and 
$h$ map $X$ to $Y$. Now, define the map $H:X \times I \rightarrow Y$ by
\[
H(x,t) = 
\begin{cases}
    F(x,2t) & \mbox{if } 0 \leq t \leq \frac{1}{2} \\
    G(x,2t-1) & \mbox{if } \frac{1}{2} < t \leq 1
\end{cases}.
\]
This map is continuous by construction. The only interesting point is $t =
\nicefrac{1}{2}$ where it is continuous since $F(x,1) = g(x) = G(x, 0)$. It
follows that $f \simeq h$.

\end{solution}

\part Show that a map homotopic to a homotopy equivalence is a homotopy
equivalence.

\begin{solution}
%
Suppose that $f: X \rightarrow Y$ is a homotopy equivalence with the homotopy
inverse $g:Y \rightarrow X$ and that $h \simeq f$ for some $h: X \rightarrow Y$.
Then, there exists a family $\{f_t:X\rightarrow Y\}_{t \in I}$ connecting $h$ to 
$f$.

Now, consider the family $\{g \circ f_t:X \rightarrow X\}_{t \in I}$. This
family connects $g \circ h$ to $g \circ f \simeq \mathbb{1}_X$. By part (b), $h
\simeq f$ if and only if $f \simeq h$ so that $h \circ g \simeq f \circ g \simeq
\mathbb{1}_Y$. We have therefore shown that $h:X \rightarrow Y$ is also a 
homotopy equivalence.

\end{solution}

\end{parts}